different CPO-definition (#66) and worked on nda_H function

untimed/CaseStudy/NDA.thy
@@ -14,16 +14,16 @@ type_synonym 'm SPS = "'m SPF uspec"
 section \<open>Non Deterministic Case \<close>
 
 (* FYI: Non-deterministic version *)
-typedef ('state::type, 'm::message) NDA = 
-  "{f::(('state \<times>(channel \<rightharpoonup> 'm)) \<Rightarrow> (('state \<times> 'm SB) set)) \<times> ('state \<times> 'm SB) set \<times> channel set \<times> channel set. True}"
-  by blast
-
+cpodef ('state::type, 'm::message) NDA = 
+  "{f::(('state \<times>(channel \<rightharpoonup> 'm)) \<Rightarrow> (('state \<times> 'm SB) set rev)) \<times> ('state \<times> 'm SB) set rev \<times> channel set discr \<times> channel set discr. True}"
+  by auto
+(*
 (* relation based on transition function and initial set *)
 instantiation NDA :: (type, message) po
 begin
   fun below_NDA :: "('a, 'b) NDA \<Rightarrow> ('a, 'b) NDA \<Rightarrow> bool" where
-  "below_NDA n1 n2 = ((fst (Rep_NDA n1) \<sqsubseteq>  fst (Rep_NDA n2))  (* Transition function is subset *)
-                  \<and>   (fst (snd (Rep_NDA n1)) \<sqsubseteq>  fst (snd (Rep_NDA n2)))  (* Initial states subset *)
+  "below_NDA n1 n2 = ((fst (Rep_NDA n2) \<sqsubseteq>  fst (Rep_NDA n1))  (* Transition function is subset. NOTICE: Reversed *)
+                  \<and>   (fst (snd (Rep_NDA n2)) \<sqsubseteq>  fst (snd (Rep_NDA n1)))  (* Initial states subset. NOTICE: Reversed *)
                   \<and>   (fst (snd (snd (Rep_NDA n1))) =  fst (snd (snd (Rep_NDA n2))))  (* input domain identical *)
                   \<and>   (     (snd (snd (snd (Rep_NDA n1)))) =  (snd (snd (snd (Rep_NDA n2))))) )" (* output domain identical *)
 
@@ -40,47 +40,90 @@ instance NDA :: (type, message) cpo
   apply (rule, rule is_lubI)
   sorry
 
+*)
 
-definition ndaTransition :: "('s, 'm::message) NDA \<rightarrow> (('s \<times>(channel \<rightharpoonup> 'm)) \<Rightarrow> (('s \<times> 'm SB) set))" where
+
+definition ndaTransition :: "('s, 'm::message) NDA \<rightarrow> (('s \<times>(channel \<rightharpoonup> 'm)) \<Rightarrow> (('s \<times> 'm SB) set rev))" where
 "ndaTransition \<equiv> \<Lambda> nda. fst (Rep_NDA nda)"
 
-definition ndaInitialState :: "('s, 'm::message) NDA \<rightarrow> ('s \<times> 'm SB) set" where
-"ndaInitialState = undefined"
+definition ndaInitialState :: "('s, 'm::message) NDA \<rightarrow> ('s \<times> 'm SB) set rev" where
+"ndaInitialState = (\<Lambda> nda. fst (snd (Rep_NDA nda)))"
 
-definition ndaDom :: "('s, 'm::message) NDA \<rightarrow> channel set" where
-"ndaDom = undefined" (* todo *)
+definition ndaDom :: "('s, 'm::message) NDA \<rightarrow> channel set discr" where
+"ndaDom = (\<Lambda> nda. fst (snd (snd (Rep_NDA nda))))"
 
-definition ndaRan :: "('s, 'm::message) NDA \<rightarrow> channel set" where
-"ndaRan = undefined" (* todo *)
+definition ndaRan :: "('s, 'm::message) NDA \<rightarrow> channel set discr" where
+"ndaRan =  (\<Lambda> nda. snd (snd (snd (Rep_NDA nda))))" 
 
 
-
+(* See: https://git.rwth-aachen.de/montibelle/automaton/core/issues/59 *)
 definition spsFix :: "('a \<rightarrow> 'a) \<rightarrow> 'a" where
 "spsFix = undefined"  (* Die ganze function ist natürlich grober unsinn *)
 
 (* like spfStep, only on SPS *)
-definition spsStep :: "channel set \<Rightarrow> channel set \<Rightarrow> ((channel\<rightharpoonup>'m::message) \<Rightarrow> 'm SPS) \<rightarrow> 'm SPS" where
-"spsStep cin cout \<equiv> undefined"
+fun spsStep :: "channel set discr \<Rightarrow> channel set discr \<Rightarrow> ((channel\<rightharpoonup>'m::message) \<Rightarrow> 'm SPS) \<rightarrow> 'm SPS" where
+"spsStep (Discr cin) (Discr cout) = undefined"
 
 
 (* ToDo *)
-definition spsHelper:: "'s \<Rightarrow> (('s \<times>'e) \<Rightarrow> ('s \<times> 'm::message SB) set) \<rightarrow> ('s \<Rightarrow> 'm SPS) \<rightarrow> ('e \<Rightarrow> 'm SPS)" where
+definition spsHelper:: "'s \<Rightarrow> (('s \<times>'e) \<Rightarrow> ('s \<times> 'm::message SB) set rev) \<rightarrow> ('s \<Rightarrow> 'm SPS) \<rightarrow> ('e \<Rightarrow> 'm SPS)" where
 "spsHelper s \<equiv> undefined (* \<Lambda> h. (\<lambda> e. (h (fst (f (s,e))))) *)"
 
 (* Similar to Rum96 *)
 definition nda_h :: "('s::type, 'm::message) NDA \<rightarrow> ('s \<Rightarrow> 'm SPS)" where
 "nda_h \<equiv>  \<Lambda> nda. spsFix\<cdot>(\<Lambda> h. (\<lambda>s. spsStep (ndaDom\<cdot>nda)(ndaRan\<cdot>nda)\<cdot>(spsHelper s\<cdot>(ndaTransition\<cdot>nda)\<cdot>h)))"
 
+definition setrevImage :: "('a \<Rightarrow> 'b) \<Rightarrow> 'a set rev \<rightarrow> 'b set rev" where
+"setrevImage = undefined"
+
+(* See: https://git.rwth-aachen.de/montibelle/automaton/core/issues/57 *)
+definition uspecImage:: "('m \<Rightarrow> 'n) \<Rightarrow> 'm uspec \<rightarrow> 'n uspec" where
+"uspecImage = undefined"
+
+(* see: https://git.rwth-aachen.de/montibelle/automaton/core/issues/58 *)
+definition uspecUnion:: "'m uspec \<rightarrow> 'm uspec \<rightarrow> 'm uspec" where
+"uspecUnion = undefined"
+
+
+(* Takes an tupel of the initial-state/output message... and returns the corresponding SPS *)
+fun helper:: "('s \<times> 'm::message SB) \<Rightarrow> ('s::type, 'm::message) NDA \<rightarrow> 'm SPS" where
+"helper (state, output) = (\<Lambda> nda. uspecImage (Rep_cfun (spfConc output))\<cdot>((nda_h\<cdot>nda) state))"
+
+
+definition nda_H_helper :: "('s, 'm::message) NDA \<rightarrow> 'm SPS set rev" where
+"nda_H_helper \<equiv> \<Lambda> nda. (setrevImage (\<lambda>t. helper t\<cdot>nda)\<cdot>(ndaInitialState\<cdot>nda))"
+
+(* This function also prepends the first SB ... *)
+(* But basically she just calls h *)
+definition nda_H :: "('s, 'm::message) NDA \<rightarrow> 'm SPS" where
+"nda_H \<equiv> \<Lambda> nda. Abs_uspec (setrevImage helper\<cdot>(ndaInitialState\<cdot>nda))"
+
+
+
+
+
+lemma nda_rep_cont[simp]: "cont Rep_NDA"
+proof -
+  obtain nn :: "(('a, 'b) NDA \<Rightarrow> ('a \<times> (channel \<Rightarrow> 'b option) \<Rightarrow> ('a \<times> 'b stream\<^sup>\<Omega>) set rev) \<times> ('a \<times> 'b stream\<^sup>\<Omega>) set rev \<times> channel set discr \<times> channel set discr) \<Rightarrow> nat \<Rightarrow> ('a, 'b) NDA" where
+    f1: "\<forall>f. chain (nn f) \<and> \<not> range (\<lambda>n. f (nn f n)) <<| f (Lub (nn f)) \<or> cont f"
+using contI by moura
+  have "Rep_NDA (Abs_NDA (\<Squnion>n. Rep_NDA (nn Rep_NDA n))) = (\<Squnion>n. Rep_NDA (nn Rep_NDA n))"
+    using Abs_NDA_inverse by blast
+then show ?thesis
+  using f1 by (metis (no_types) below_NDA_def lub_NDA po_class.chain_def thelubE)
+qed
+
+
+lemma "cont (\<lambda>nda. fst (Rep_NDA nda))"
+  by simp
+
+
+
 lemma "cont (\<lambda> nda. spsFix\<cdot>(\<Lambda> h. (\<lambda>s. spsStep some suff\<cdot>(spsHelper s\<cdot>(ndaTransition\<cdot>nda)\<cdot>h))))"
   by simp
 
 lemma "cont (\<lambda> h. (\<lambda>s. spsStep (ndaDom\<cdot>nda)(ndaRan\<cdot>nda)\<cdot>(spsHelper s\<cdot>(ndaTransition\<cdot>nda)\<cdot>h)))"
   by simp
-(* This function also prepends the first SB ... *)
-(* But basically she just calls h *)
-definition nda_H :: "('s, 'm::message) NDA \<rightarrow> 'm SPF set" where
-"nda_H \<equiv> \<Lambda> nda. undefined"
-
 
 
 end
